ulib/mk_int.sh
@@ -1,6 +1,6 @@
 #!/bin/bash
 
-for i in 8 16 31 32 63 64; do
+for i in 8 16 31 32 63 64 128; do
   f=FStar.Int$i.fst
   cat > $f <<EOF
 module FStar.Int$i
@@ -10,9 +10,20 @@ let n = $i
 
 EOF
   cat FStar.IntN.fstp >> $f
+  if [ $i -eq 128 ]; then
+      cat >> $f <<EOF
+
+val mul_wide: a:Int64.t -> b:Int64.t -> Pure t
+  (requires True)
+  (ensures (fun c -> v c = Int64.v a * Int64.v b))
+let mul_wide a b = 
+  assume (size (Int64.v a * Int64.v b) n);
+  Mk ((Int64.v a) * (Int64.v b))
+EOF
+  fi
 done
 
-for i in 8 16 31 32 63 64; do
+for i in 8 16 31 32 63 64 128; do
   f=FStar.UInt$i.fst
   cat > $f <<EOF
 module FStar.UInt$i
@@ -25,4 +36,17 @@ EOF
   if [ $i -eq 8 ]; then
     echo "type byte = t" >> $f
   fi
+  if [ $i -eq 128 ]; then
+      cat >> $f <<EOF
+
+val mul_wide: a:UInt64.t -> b:UInt64.t -> Pure t
+  (requires True)
+  (ensures (fun c -> v c = UInt64.v a * UInt64.v b))
+let mul_wide a b = 
+  assume (size (UInt64.v a * UInt64.v b) n);
+  Mk ((UInt64.v a) * (UInt64.v b))
+EOF
+  fi
 done
+
+sed -i 's/UInt32.//g' FStar.UInt32.fst
